inhale_exhale_wildcard_2.bpl
@@ -17,7 +17,7 @@
 // Before -> function state(Heap: HeapType, Mask: MaskType): bool;
 // Afterwards
 
-  function state(Heap: HeapType, Mask: MaskType, BMask: BMaskType): bool;
+  function state(Heap: HeapType, Mask: MaskType): bool;
 
 // ==================================================
 // Preamble of Heap module.
@@ -36,45 +36,45 @@ axiom (forall o: Ref, f: (Field NormalField Ref), Heap: HeapType ::
 );
 function succHeap(Heap0: HeapType, Heap1: HeapType): bool;
 function succHeapTrans(Heap0: HeapType, Heap1: HeapType): bool;
-function IdenticalOnKnownLocations(Heap: HeapType, ExhaleHeap: HeapType, Mask: MaskType, BMask: BMaskType): bool;
+function IdenticalOnKnownLocations(Heap: HeapType, ExhaleHeap: HeapType, Mask: MaskType): bool;
 function IsPredicateField<A, B>(f_1: (Field A B)): bool;
 function IsWandField<A, B>(f_1: (Field A B)): bool;
 function getPredicateId<A, B>(f_1: (Field A B)): int;
 // Frame all locations with direct permissions
-axiom (forall <A, B> Heap: HeapType, ExhaleHeap: HeapType, Mask: MaskType, BMask: BMaskType, o: Ref, f_2: (Field A B) ::
-  { IdenticalOnKnownLocations(Heap, ExhaleHeap, Mask, BMask), ExhaleHeap[o, f_2] }
-  IdenticalOnKnownLocations(Heap, ExhaleHeap, Mask, BMask) ==> HasDirectPerm(Mask, BMask, o, f_2) ==> Heap[o, f_2] == ExhaleHeap[o, f_2]
+axiom (forall <A, B> Heap: HeapType, ExhaleHeap: HeapType, Mask: MaskType, o: Ref, f_2: (Field A B) ::
+  { IdenticalOnKnownLocations(Heap, ExhaleHeap, Mask), ExhaleHeap[o, f_2] }
+  IdenticalOnKnownLocations(Heap, ExhaleHeap, Mask) ==> HasDirectPerm(Mask, o, f_2) ==> Heap[o, f_2] == ExhaleHeap[o, f_2]
 );
 // Frame all predicate mask locations of predicates with direct permission
-axiom (forall <C> Heap: HeapType, ExhaleHeap: HeapType, Mask: MaskType, BMask: BMaskType, pm_f: (Field C FrameType) ::
-  { IdenticalOnKnownLocations(Heap, ExhaleHeap, Mask, BMask), IsPredicateField(pm_f), ExhaleHeap[null, PredicateMaskField(pm_f)] }
-  IdenticalOnKnownLocations(Heap, ExhaleHeap, Mask, BMask) ==> HasDirectPerm(Mask, BMask, null, pm_f) && IsPredicateField(pm_f) ==> Heap[null, PredicateMaskField(pm_f)] == ExhaleHeap[null, PredicateMaskField(pm_f)]
+axiom (forall <C> Heap: HeapType, ExhaleHeap: HeapType, Mask: MaskType, pm_f: (Field C FrameType) ::
+  { IdenticalOnKnownLocations(Heap, ExhaleHeap, Mask), IsPredicateField(pm_f), ExhaleHeap[null, PredicateMaskField(pm_f)] }
+  IdenticalOnKnownLocations(Heap, ExhaleHeap, Mask) ==> HasDirectPerm(Mask, null, pm_f) && IsPredicateField(pm_f) ==> Heap[null, PredicateMaskField(pm_f)] == ExhaleHeap[null, PredicateMaskField(pm_f)]
 );
 // Frame all locations with known folded permissions
-axiom (forall <C> Heap: HeapType, ExhaleHeap: HeapType, Mask: MaskType, BMask: BMaskType, pm_f: (Field C FrameType) ::
-  { IdenticalOnKnownLocations(Heap, ExhaleHeap, Mask, BMask), ExhaleHeap[null, pm_f], IsPredicateField(pm_f) }
-  IdenticalOnKnownLocations(Heap, ExhaleHeap, Mask, BMask) ==> HasDirectPerm(Mask, BMask, null, pm_f) && IsPredicateField(pm_f) ==> (forall <A, B> o2: Ref, f_2: (Field A B) ::
+axiom (forall <C> Heap: HeapType, ExhaleHeap: HeapType, Mask: MaskType, pm_f: (Field C FrameType) ::
+  { IdenticalOnKnownLocations(Heap, ExhaleHeap, Mask), ExhaleHeap[null, pm_f], IsPredicateField(pm_f) }
+  IdenticalOnKnownLocations(Heap, ExhaleHeap, Mask) ==> HasDirectPerm(Mask, null, pm_f) && IsPredicateField(pm_f) ==> (forall <A, B> o2: Ref, f_2: (Field A B) ::
     { ExhaleHeap[o2, f_2] }
     Heap[null, PredicateMaskField(pm_f)][o2, f_2] ==> Heap[o2, f_2] == ExhaleHeap[o2, f_2]
   )
 );
 // Frame all wand mask locations of wands with direct permission
-axiom (forall <C> Heap: HeapType, ExhaleHeap: HeapType, Mask: MaskType, BMask: BMaskType, pm_f: (Field C FrameType) ::
-  { IdenticalOnKnownLocations(Heap, ExhaleHeap, Mask, BMask), IsWandField(pm_f), ExhaleHeap[null, WandMaskField(pm_f)] }
-  IdenticalOnKnownLocations(Heap, ExhaleHeap, Mask, BMask) ==> HasDirectPerm(Mask, BMask, null, pm_f) && IsWandField(pm_f) ==> Heap[null, WandMaskField(pm_f)] == ExhaleHeap[null, WandMaskField(pm_f)]
+axiom (forall <C> Heap: HeapType, ExhaleHeap: HeapType, Mask: MaskType, pm_f: (Field C FrameType) ::
+  { IdenticalOnKnownLocations(Heap, ExhaleHeap, Mask), IsWandField(pm_f), ExhaleHeap[null, WandMaskField(pm_f)] }
+  IdenticalOnKnownLocations(Heap, ExhaleHeap, Mask) ==> HasDirectPerm(Mask, null, pm_f) && IsWandField(pm_f) ==> Heap[null, WandMaskField(pm_f)] == ExhaleHeap[null, WandMaskField(pm_f)]
 );
 // Frame all locations in the footprint of magic wands
-axiom (forall <C> Heap: HeapType, ExhaleHeap: HeapType, Mask: MaskType, BMask: BMaskType, pm_f: (Field C FrameType) ::
-  { IdenticalOnKnownLocations(Heap, ExhaleHeap, Mask, BMask), IsWandField(pm_f) }
-  IdenticalOnKnownLocations(Heap, ExhaleHeap, Mask, BMask) ==> HasDirectPerm(Mask, BMask, null, pm_f) && IsWandField(pm_f) ==> (forall <A, B> o2: Ref, f_2: (Field A B) ::
+axiom (forall <C> Heap: HeapType, ExhaleHeap: HeapType, Mask: MaskType, pm_f: (Field C FrameType) ::
+  { IdenticalOnKnownLocations(Heap, ExhaleHeap, Mask), IsWandField(pm_f) }
+  IdenticalOnKnownLocations(Heap, ExhaleHeap, Mask) ==> HasDirectPerm(Mask, null, pm_f) && IsWandField(pm_f) ==> (forall <A, B> o2: Ref, f_2: (Field A B) ::
     { ExhaleHeap[o2, f_2] }
     Heap[null, WandMaskField(pm_f)][o2, f_2] ==> Heap[o2, f_2] == ExhaleHeap[o2, f_2]
   )
 );
 // All previously-allocated references are still allocated
-axiom (forall Heap: HeapType, ExhaleHeap: HeapType, Mask: MaskType, BMask: BMaskType, o: Ref ::
-  { IdenticalOnKnownLocations(Heap, ExhaleHeap, Mask, BMask), ExhaleHeap[o, $allocated] }
-  IdenticalOnKnownLocations(Heap, ExhaleHeap, Mask, BMask) ==> Heap[o, $allocated] ==> ExhaleHeap[o, $allocated]
+axiom (forall Heap: HeapType, ExhaleHeap: HeapType, Mask: MaskType, o: Ref ::
+  { IdenticalOnKnownLocations(Heap, ExhaleHeap, Mask), ExhaleHeap[o, $allocated] }
+  IdenticalOnKnownLocations(Heap, ExhaleHeap, Mask) ==> Heap[o, $allocated] ==> ExhaleHeap[o, $allocated]
 );
 // Updated Heaps are Successor Heaps
 axiom (forall <A, B> Heap: HeapType, o: Ref, f_2: (Field A B), v: B ::
@@ -82,9 +82,9 @@ axiom (forall <A, B> Heap: HeapType, o: Ref, f_2: (Field A B), v: B ::
   succHeap(Heap, Heap[o, f_2:=v])
 );
 // IdenticalOnKnownLocations Heaps are Successor Heaps
-axiom (forall Heap: HeapType, ExhaleHeap: HeapType, Mask: MaskType, BMask: BMaskType ::
-  { IdenticalOnKnownLocations(Heap, ExhaleHeap, Mask, BMask) }
-  IdenticalOnKnownLocations(Heap, ExhaleHeap, Mask, BMask) ==> succHeap(Heap, ExhaleHeap)
+axiom (forall Heap: HeapType, ExhaleHeap: HeapType, Mask: MaskType ::
+  { IdenticalOnKnownLocations(Heap, ExhaleHeap, Mask) }
+  IdenticalOnKnownLocations(Heap, ExhaleHeap, Mask) ==> succHeap(Heap, ExhaleHeap)
 );
 // Successor Heaps are Transitive Successor Heaps
 axiom (forall Heap0: HeapType, Heap1: HeapType ::
@@ -101,28 +101,22 @@ axiom (forall Heap0: HeapType, Heap1: HeapType, Heap2: HeapType ::
 // Preamble of Permission module.
 // ==================================================
 
-type Perm = real;
+type Pair A B;
+function pair<A, B>(a: A, b: B) : Pair A B;
+function fst<A, B>(p: Pair A B) : A;
+function snd<A, B>(p: Pair A B) : B;
+axiom (forall <A, B> a:A, b:B :: {pair(a,b)} fst(pair(a,b)) == a);
+axiom (forall <A, B> a:A, b:B :: {pair(a,b)} snd(pair(a,b)) == a);
+axiom (forall <A, B> p: Pair A B :: {fst(p)}{snd(p)} pair(fst(p), snd(p)) == p)
+
+tyoe Perm = Pair real bool;
 type MaskType = <A, B> [Ref, Field A B]Perm;
 var Mask: MaskType;
-// Change
-// Before (nothing)
-// Afterwards
-type BMaskType = <A, B> [Ref, Field A B]bool;
-var BMask: BMaskType;
 const ZeroMask: MaskType;
 axiom (forall <A, B> o_1: Ref, f_3: (Field A B) ::
   { ZeroMask[o_1, f_3] }
-  ZeroMask[o_1, f_3] == NoPerm
+  fst(ZeroMask[o_1, f_3]) == NoPerm && !snd(ZeroMask)
 );
-// Change
-// Before (nothing)
-// Afterwards
-const ZeroBMask: BMaskType;
-axiom (forall <A, B> o_1: Ref, f_3: (Field A B) ::
-  { ZeroBMask[o_1, f_3] }
-  !ZeroBMask[o_1, f_3]
-);
-
 type PMaskType = <A, B> [Ref, Field A B]bool;
 const ZeroPMask: PMaskType;
 axiom (forall <A, B> o_1: Ref, f_3: (Field A B) ::
@@ -132,32 +126,22 @@ axiom (forall <A, B> o_1: Ref, f_3: (Field A B) ::
 function PredicateMaskField<A>(f_4: (Field A FrameType)): Field A PMaskType;
 function WandMaskField<A>(f_4: (Field A FrameType)): Field A PMaskType;
 const NoPerm: Perm;
-axiom NoPerm == 0.000000000;
+axiom NoPerm == pair(0.000000000, false);
 const FullPerm: Perm;
-axiom FullPerm == 1.000000000;
-function Perm(a: real, b: real): Perm;
-function GoodMask(Mask: MaskType, BMask: BMaskType): bool;
-axiom (forall Heap: HeapType, Mask: MaskType, BMask: BMaskType ::
-  { state(Heap, Mask, BMask) }
-  state(Heap, Mask, BMask) ==> GoodMask(Mask, BMask)
-);
-// TODO: check if this encoding works
-axiom (forall <A, B> Mask: MaskType, BMask: BMaskType, o_1: Ref, f_3: (Field A B) ::
-  { GoodMask(Mask, BMask), Mask[o_1, f_3], BMask[o_1, f_3] }
-  GoodMask(Mask, BMask) ==> Mask[o_1, f_3] >= NoPerm && ((GoodMask(Mask, BMask) && !IsPredicateField(f_3)) && !IsWandField(f_3) ==> Mask[o_1, f_3] <= FullPerm)
+axiom FullPerm == pair(1.000000000, false);
+function Perm(a: real, b: real, b: bool): Perm;
+function GoodMask(Mask: MaskType): bool;
+axiom (forall Heap: HeapType, Mask: MaskType ::
+  { state(Heap, Mask) }
+  state(Heap, Mask) ==> GoodMask(Mask)
 );
 
-// Change
-// Before (nothing)
-// function GoodBMask(BMask: BMaskType): bool;
-// axiom (forall Heap: HeapType, Mask: MaskType, BMask: BMaskType ::
-//  { state(Heap, Mask, BMask) }
-//  state(Heap, Mask, BMask) ==> GoodBMask(BMask)
-//);
-// axiom (forall <A, B> BMask: BMaskType, o_1: Ref, f_3: (Field A B) ::
-//   { GoodBMask(BMask), BMask[o_1, f_3] }
-//   GoodBMask(BMask) ==> ((GoodBMask(BMask) && !IsPredicateField(f_3)))
-// );
+// Something missing for sWildcard?
+axiom (forall <A, B> Mask: MaskType, o_1: Ref, f_3: (Field A B) ::
+  { GoodMask(Mask), Mask[o_1, f_3]}
+  GoodMask(Mask) ==> fst(Mask[o_1, f_3]) >= NoPerm && ((fst(GoodMask(Mask)) && !IsPredicateField(f_3)) && !IsWandField(f_3) ==> fst(Mask[o_1, f_3]) <= FullPerm)
+);
+
 
 // Change 
 // Before
@@ -167,23 +151,17 @@ axiom (forall <A, B> Mask: MaskType, BMask: BMaskType, o_1: Ref, f_3: (Field A B
 //   HasDirectPerm(Mask, o_1, f_3) <==> Mask[o_1, f_3] > NoPerm
 // );
 // Afterwards
-function HasDirectPerm<A, B>(Mask: MaskType, BMask: BMaskType, o_1: Ref, f_3: (Field A B)): bool;
-axiom (forall <A, B> Mask: MaskType, BMask: BMaskType, o_1: Ref, f_3: (Field A B) ::
-  { HasDirectPerm(Mask, BMask, o_1, f_3) }
-  HasDirectPerm(Mask, BMask, o_1, f_3) <==> Mask[o_1, f_3] > NoPerm || (Mask[o_1, f_3] == NoPerm && BMask[o_1, f_3])
+function HasDirectPerm<A, B>(Mask: MaskType, o_1: Ref, f_3: (Field A B)): bool;
+axiom (forall <A, B> Mask: MaskType, o_1: Ref, f_3: (Field A B) ::
+  { HasDirectPerm(Mask, o_1, f_3) }
+  HasDirectPerm(Mask, o_1, f_3) <==> fst(Mask[o_1, f_3]) > NoPerm || (fst(Mask[o_1, f_3]) == NoPerm && snd(Mask[o_1, f_3]))
 );
+
 function sumMask(ResultMask: MaskType, SummandMask1: MaskType, SummandMask2: MaskType): bool;
 axiom (forall <A, B> ResultMask: MaskType, SummandMask1: MaskType, SummandMask2: MaskType, o_1: Ref, f_3: (Field A B) ::
   { sumMask(ResultMask, SummandMask1, SummandMask2), ResultMask[o_1, f_3] } { sumMask(ResultMask, SummandMask1, SummandMask2), SummandMask1[o_1, f_3] } { sumMask(ResultMask, SummandMask1, SummandMask2), SummandMask2[o_1, f_3] }
-  sumMask(ResultMask, SummandMask1, SummandMask2) ==> ResultMask[o_1, f_3] == SummandMask1[o_1, f_3] + SummandMask2[o_1, f_3]
-);
-// Change 
-// Before (nothing)
-// Afterwards
-function sumBMask(ResultBMask: BMaskType, SummandBMask1: BMaskType, SummandBMask2: BMaskType): bool;
-axiom (forall <A, B> ResultBMask: BMaskType, SummandBMask1: BMaskType, SummandBMask2: BMaskType, o_1: Ref, f_3: (Field A B) ::
-  { sumBMask(ResultBMask, SummandBMask1, SummandBMask2), ResultBMask[o_1, f_3] } { sumBMask(ResultBMask, SummandBMask1, SummandBMask2), SummandBMask1[o_1, f_3] } { sumBMask(ResultBMask, SummandBMask1, SummandBMask2), SummandBMask2[o_1, f_3] }
-  sumBMask(ResultBMask, SummandBMask1, SummandBMask2) ==> ResultBMask[o_1, f_3] == SummandBMask1[o_1, f_3] || SummandBMask2[o_1, f_3]
+  sumMask(ResultMask, SummandMask1, SummandMask2) ==> fst(ResultMask[o_1, f_3]) == fst(SummandMask1[o_1, f_3]) + fst(SummandMask2[o_1, f_3]) 
+                                                      && snd(ResultMask[o_1, f_3]) == snd(SummandMask1[o_1, f_3]) || snd(SummandMask2[o_1, f_3])
 );
 
 // ==================================================
@@ -201,9 +179,10 @@ function CombineFrames(a_1: FrameType, b_1: FrameType): FrameType;
 // Definition of conditional frame fragments
 // ==================================================
 
+//Change
 axiom (forall p: Perm, f_5: FrameType ::
   { ConditionalFrame(p, f_5) }
-  ConditionalFrame(p, f_5) == (if p > 0.000000000 then f_5 else EmptyFrame)
+  ConditionalFrame(p, f_5) == (if fst(p) > 0.000000000 then f_5 else EmptyFrame)
 );
 // Function for recording enclosure of one predicate instance in another
 function InsidePredicate<A, B>(p: (Field A FrameType), v_1: FrameType, q: (Field B FrameType), w: FrameType): bool;
@@ -231,7 +210,7 @@ axiom !IsWandField(f_6);
 // ==================================================
 
 procedure test(x: Ref) returns ()
-  modifies Heap, Mask, BMask;
+  modifies Heap, Mask;
 {
   // Change
   // Before -> var sWildcard: real where sWildcard > NoPerm;
@@ -239,17 +218,12 @@ procedure test(x: Ref) returns ()
   // Afterwards (Nothing)
   var PostHeap: HeapType;
   var PostMask: MaskType;
-  var PostBMask: BMaskType;
-  // Change
-  // Before (nothing)
-  // Afterwards
-  var BPostMask: BMaskType;
   var v_2: int;
   var ExhaleHeap: HeapType;
   
   // -- Initializing the state
     Mask := ZeroMask;
-    assume state(Heap, Mask, BMask);
+    assume state(Heap, Mask);
   
   // -- Assumptions about method arguments
     assume Heap[x, $allocated];
@@ -262,31 +236,19 @@ procedure test(x: Ref) returns ()
     // assume perm > NoPerm ==> x != null;
     // Mask[x, f_6] := Mask[x, f_6] + perm;
     // Afterwards
-    BMask[x, f_6] := true;
-    assume state(Heap, Mask, BMask);
+    snd(Mask[x, f_6]) := true;
+    assume state(Heap, Mask);
   
   // -- Initializing of old state
     
     // -- Initializing the old state
       assume Heap == old(Heap);
       assume Mask == old(Mask);
-      // Change
-      // Before (nothing)
-      // Afterwards
-      assume BMask == old(BMask);
   PostHeap := Heap;
   PostMask := Mask;
-  // Change
-  // Before (nothing)
-  // Afterwards
-  PostBMask := BMask;
   havoc PostHeap;
   PostMask := ZeroMask;
-  // Change
-  // Before (nothing)
-  // Afterwards
-  PostBMask := ZeroBMask;
-  assume state(PostHeap, PostMask, PostBMask);
+  assume state(PostHeap, PostMask);
   if (*) {
     // Checked inhaling of postcondition to check definedness
     // Change
@@ -296,12 +258,12 @@ procedure test(x: Ref) returns ()
     // assume perm >= NoPerm;
     // assume perm > NoPerm ==> x != null;
     // PostMask[x, f_6] := PostMask[x, f_6] + perm;
-    assume state(PostHeap, PostMask, PostBMask);
-    assume state(PostHeap, PostMask, PostBMask);
+    assume state(PostHeap, PostMask);
+    assume state(PostHeap, PostMask);
     // Afterwards
-    PostBMask[x, f_6] := true;
-    assume state(PostHeap, PostMask, PostBMask);
-    assume state(PostHeap, PostMask, PostBMask);
+    snd(PostMask[x, f_6]) := true;
+    assume state(PostHeap, PostMask);
+    assume state(PostHeap, PostMask);
     // Stop execution
     assume false;
   }
@@ -310,10 +272,10 @@ procedure test(x: Ref) returns ()
     
     // -- Check definedness of x.f
       assert {:msg "  Assignment might fail. There might be insufficient permission to access x.f. (test.vpr@7.5) [3]"}
-        HasDirectPerm(Mask, BMask, x, f_6);
-      assume state(Heap, Mask, BMask);
+        HasDirectPerm(Mask, x, f_6);
+      assume state(Heap, Mask);
     v_2 := Heap[x, f_6];
-    assume state(Heap, Mask, BMask);
+    assume state(Heap, Mask);
   
   // -- Exhaling postcondition
     // Phase 1: pure assertions and fixed permissions
@@ -326,6 +288,6 @@ procedure test(x: Ref) returns ()
 
     // Finish exhale
     havoc ExhaleHeap;
-    assume IdenticalOnKnownLocations(Heap, ExhaleHeap, Mask, BMask);
+    assume IdenticalOnKnownLocations(Heap, ExhaleHeap, Mask);
     Heap := ExhaleHeap;
 }
